feat: add preorder on magma laws (#135)
* feat: add preorder on magma laws

This builds on the `MagmaLaw` structure defined in #113 and thus depends on it.

* integrate with definitions from #123

* add equivalence suggested by @codyroux

* remove whitespace

* add suggestions from @madvorak

* more style changes suggested by @madvorak

* minor improvements

---------

Co-authored-by: Pietro Monticone <38562595+pitmonticone@users.noreply.github.com>

equational_theories/Completeness.lean
@@ -4,6 +4,8 @@
 import equational_theories.FreeMagma
 import Mathlib.Data.Set.Defs
 
+open FreeMagma
+
 structure MagmaLaw (α : Type) where
   lhs : FreeMagma α
   rhs : FreeMagma α
@@ -23,6 +25,8 @@ def Ctx α := Set (MagmaLaw α)
 
 -- FIXME: figure out how to remove this.
 instance Ctx.Membership α : Membership (MagmaLaw α) (Ctx α) := ⟨ Set.instMembership.mem ⟩
+
+instance {α : Type} : Singleton (MagmaLaw α) (Ctx α) := ⟨Set.singleton⟩
 
 section DeriveDef
 
@@ -44,7 +48,7 @@ inductive derive {α} : Ctx α → MagmaLaw α → Type :=
 end DeriveDef
 
 def satisfiesPhi {α G : Type} [Magma G] (φ : α → G) (E : MagmaLaw α) : Prop :=
-  evalInMagma φ E.lhs = evalInMagma φ E.rhs
+  E.lhs.evalInMagma φ = E.rhs.evalInMagma φ
 
 def satisfies {α : Type} (G : Type) [Magma G] (E : MagmaLaw α) := ∀ (φ : α → G), satisfiesPhi φ E
 
