equational_theories/Preorder.lean
@@ -1,0 +1,35 @@
+import Mathlib.Order.Defs
+import Mathlib.Data.Set.Basic
+import equational_theories.Completeness
+
+namespace MagmaLaw
+
+variable {α : Type}
+
+/--
+A magma law `l₁` implies a law `l₂` if in any Magma `G` where `l₁` holds, `l₂` also holds.
+
+We have to explicitly quantify the type `G` and the Magma instance `[Magma G]` instead of
+using them as parameters so that the implication holds in any Magma `G`.
+-/
+def implies (l₁ l₂ : MagmaLaw α) := ∀ {G : Type} [Magma G],
+  satisfies G l₁ → satisfies G l₂
+
+instance : LE (MagmaLaw α) where
+  le l₁ l₂ := l₁.implies l₂
+
+theorem implies_refl (l : MagmaLaw α) : l ≤ l := fun {G} [Magma G] a ↦ a
+
+theorem implies_trans {l₁ l₂ l₃ : MagmaLaw α} : l₁ ≤ l₂ → l₂ ≤ l₃ → l₁ ≤ l₃ := by
+  intro h₁ h₂ G inst h
+  dsimp only [satisfies, satisfiesPhi] at *
+  exact h₂ (h₁ h)
+
+instance : Preorder (MagmaLaw α) where
+  le_refl := implies_refl
+  le_trans := fun _ _ _ ↦ implies_trans
+
+theorem implies_eq_singleton_models {l₁ l₂ : MagmaLaw α} : l₁ ≤ l₂ ↔ {l₁} ⊧ l₂ := by
+  simp only [LE.le, implies, models, satisfiesSet, Ctx, Set.mem_singleton_iff, forall_eq]
+
+end MagmaLaw
